\subsection{Problem 5: Integral with Inverse Sine}

\begin{problem}
Using the substitution $x = \tan^2 \theta$, evaluate
\[
\int_{0}^{1} \sin^{-1} \sqrt{\frac{x}{1+x}} \,dx.
\]
\end{problem}

\begin{hint}
After making the substitution, simplify the integrand. You may need to use trigonometric identities. Consider the relationship between $\sin^{-1}$ and the substitution variable.
\end{hint}

\subsection{Solution to Problem 5: Integral with Inverse Sine}

\begin{solution}
Let $x = \tan^2 \theta$, so $dx = 2\tan\theta \sec^2\theta \, d\theta = 2\tan\theta(1 + \tan^2\theta) \, d\theta$.

When $x = 0$, $\theta = 0$; when $x = 1$, $\theta = \pi/4$.

The integrand becomes:
\[
\sin^{-1}\sqrt{\frac{x}{1+x}} = \sin^{-1}\sqrt{\frac{\tan^2\theta}{1+\tan^2\theta}} = \sin^{-1}\sqrt{\frac{\tan^2\theta}{\sec^2\theta}} = \sin^{-1}|\sin\theta| = \sin^{-1}(\sin\theta) = \theta
\]
for $\theta \in [0, \pi/4]$.

Therefore:
\[
\int_0^1 \sin^{-1}\sqrt{\frac{x}{1+x}} \, dx = \int_0^{\pi/4} \theta \cdot 2\tan\theta \sec^2\theta \, d\theta
\]
Using integration by parts with $u = \theta$, $dv = 2\tan\theta \sec^2\theta \, d\theta$:
\[
= \left[\theta \tan^2\theta\right]_0^{\pi/4} - \int_0^{\pi/4} \tan^2\theta \, d\theta = \frac{\pi}{4} - \int_0^{\pi/4} (\sec^2\theta - 1) \, d\theta
\]
\[
= \frac{\pi}{4} - [\tan\theta - \theta]_0^{\pi/4} = \frac{\pi}{4} - (1 - \frac{\pi}{4}) = \frac{\pi}{2} - 1
\]
\end{solution}

\begin{takeaways}
\begin{itemize}
    \item Substitution $x = \tan^2\theta$ simplifies $\sqrt{x/(1+x)}$ to $|\sin\theta|$
    \item For $\theta \in [0, \pi/4]$, we have $\sin^{-1}(\sin\theta) = \theta$
    \item Integration by parts: differentiate the polynomial part, integrate the trigonometric part
\end{itemize}
\end{takeaways}

