\subsection{Solution to Problem 6: Integral with Cotangent}

\begin{solution}
\textbf{(i)} Write $I_n = \int_{\pi/4}^{\pi/2} \cot^{2n}\theta \, d\theta = \int_{\pi/4}^{\pi/2} \cot^{2n-2}\theta \cdot \cot^2\theta \, d\theta$.

Using $\cot^2\theta = \csc^2\theta - 1$:
\[
I_n = \int_{\pi/4}^{\pi/2} \cot^{2n-2}\theta (\csc^2\theta - 1) \, d\theta = \int_{\pi/4}^{\pi/2} \cot^{2n-2}\theta \csc^2\theta \, d\theta - I_{n-1}
\]

For the first integral, let $u = \cot\theta$, so $du = -\csc^2\theta \, d\theta$:
\[
\int_{\pi/4}^{\pi/2} \cot^{2n-2}\theta \csc^2\theta \, d\theta = -\int_1^0 u^{2n-2} \, du = \int_0^1 u^{2n-2} \, du = \frac{1}{2n-1}
\]

Therefore: $I_n = \frac{1}{2n-1} - I_{n-1}$.

\textbf{(ii)} First, $I_0 = \int_{\pi/4}^{\pi/2} d\theta = \frac{\pi}{4}$.

Using the recurrence: $I_1 = \frac{1}{1} - I_0 = 1 - \frac{\pi}{4}$.

Then: $I_2 = \frac{1}{3} - I_1 = \frac{1}{3} - (1 - \frac{\pi}{4}) = \frac{\pi}{4} - \frac{2}{3}$.
\end{solution}

\begin{takeaways}
\begin{itemize}
    \item Recurrence: Use $\cot^2\theta = \csc^2\theta - 1$ to relate $I_n$ and $I_{n-1}$
    \item Substitution: $u = \cot\theta$ converts $\cot^{2n-2}\theta \csc^2\theta \, d\theta$ to $u^{2n-2} \, du$
    \item Base case: $I_0 = \pi/4$ (integral of 1 over the interval)
\end{itemize}
\end{takeaways}

