\subsection{Solution to Problem 17: Integration with Recurrence Relations}

\begin{solution}
\textbf{(i)} Using integration by parts with $u = \sin^{n-1}\theta$ and $dv = \sin\theta \, d\theta$:
\[
J_n = \int_0^{\pi/2} \sin^n\theta \, d\theta = \int_0^{\pi/2} \sin^{n-1}\theta \cdot \sin\theta \, d\theta
\]
Let $u = \sin^{n-1}\theta$, $dv = \sin\theta \, d\theta$, so $du = (n-1)\sin^{n-2}\theta \cos\theta \, d\theta$ and $v = -\cos\theta$:
\[
J_n = \left[-\sin^{n-1}\theta \cos\theta\right]_0^{\pi/2} + (n-1)\int_0^{\pi/2} \sin^{n-2}\theta \cos^2\theta \, d\theta
\]
The boundary term is 0. Using $\cos^2\theta = 1 - \sin^2\theta$:
\[
J_n = (n-1)\int_0^{\pi/2} \sin^{n-2}\theta (1 - \sin^2\theta) \, d\theta = (n-1)(J_{n-2} - J_n)
\]
Solving: $J_n = (n-1)J_{n-2} - (n-1)J_n$, so $nJ_n = (n-1)J_{n-2}$.

Therefore: $J_n = \frac{n-1}{n}J_{n-2}$.

\textbf{(ii)} Using substitution $x = \sin^2\theta$, so $dx = 2\sin\theta\cos\theta \, d\theta$ and $1-x = \cos^2\theta$:
\[
I_n = \int_0^1 x^n(1-x)^n \, dx = \int_0^{\pi/2} \sin^{2n}\theta \cos^{2n}\theta \cdot 2\sin\theta\cos\theta \, d\theta
\]
\[
= 2\int_0^{\pi/2} \sin^{2n+1}\theta \cos^{2n+1}\theta \, d\theta = 2\int_0^{\pi/2} (\sin\theta\cos\theta)^{2n+1} \, d\theta
\]
Using $\sin(2\theta) = 2\sin\theta\cos\theta$, so $\sin\theta\cos\theta = \frac{1}{2}\sin(2\theta)$:
\[
I_n = 2\int_0^{\pi/2} \left(\frac{1}{2}\sin(2\theta)\right)^{2n+1} \, d\theta = \frac{2}{2^{2n+1}}\int_0^{\pi/2} \sin^{2n+1}(2\theta) \, d\theta
\]
Let $u = 2\theta$, so $du = 2d\theta$:
\[
I_n = \frac{1}{2^{2n+1}} \int_0^{\pi} \sin^{2n+1}u \cdot \frac{du}{2} = \frac{1}{2^{2n+2}} \int_0^{\pi} \sin^{2n+1}u \, du
\]
By symmetry: $\int_0^{\pi} \sin^{2n+1}u \, du = 2\int_0^{\pi/2} \sin^{2n+1}u \, du$.

Therefore: $I_n = \frac{1}{2^{2n+2}} \cdot 2J_{2n+1} = \frac{1}{2^{2n+1}}J_{2n+1}$.

\textbf{(iii)} From part (ii): $I_n = \frac{1}{2^{2n+1}}J_{2n+1}$ and $I_{n-1} = \frac{1}{2^{2n-1}}J_{2n-1}$.

From part (i): $J_{2n+1} = \frac{2n}{2n+1}J_{2n-1}$.

Therefore:
\[
I_n = \frac{1}{2^{2n+1}} \cdot \frac{2n}{2n+1}J_{2n-1} = \frac{2n}{2n+1} \cdot \frac{1}{2^{2n+1}}J_{2n-1} = \frac{2n}{2n+1} \cdot \frac{1}{4} \cdot \frac{1}{2^{2n-1}}J_{2n-1}
\]
\[
= \frac{n}{2(2n+1)} \cdot I_{n-1} = \frac{n}{4n+2}I_{n-1}
\]
\end{solution}

\begin{takeaways}
\begin{itemize}
    \item Integration by parts: Use to derive recurrence relations for powers of trigonometric functions
    \item Substitution: $x = \sin^2\theta$ converts polynomial integrals to trigonometric integrals
    \item Combining recurrences: Use multiple recurrence relations together to prove new results
\end{itemize}
\end{takeaways}

