\subsection{Solution to Problem 28: Induction Proof for Series}

\begin{solution}
\textbf{Base case ($n = 2$):} LHS $= \frac{1}{4} = 0.25$, RHS $= \frac{1}{2} = 0.5$. So $0.25 < 0.5$ $\checkmark$

\textbf{Inductive step:} Assume true for $n = k$, i.e., $\frac{1}{2^2} + \frac{1}{3^2} + \dots + \frac{1}{k^2} < \frac{k-1}{k}$.

For $n = k+1$, we need to show:
\[
\frac{1}{2^2} + \frac{1}{3^2} + \dots + \frac{1}{k^2} + \frac{1}{(k+1)^2} < \frac{k}{k+1}
\]

By the inductive hypothesis:
\[
\frac{1}{2^2} + \frac{1}{3^2} + \dots + \frac{1}{k^2} + \frac{1}{(k+1)^2} < \frac{k-1}{k} + \frac{1}{(k+1)^2}
\]

We need: $\frac{k-1}{k} + \frac{1}{(k+1)^2} < \frac{k}{k+1}$.

This is equivalent to: $\frac{k-1}{k} < \frac{k}{k+1} - \frac{1}{(k+1)^2} = \frac{k(k+1) - 1}{(k+1)^2} = \frac{k^2 + k - 1}{(k+1)^2}$.

Cross-multiplying: $(k-1)(k+1)^2 < k(k^2 + k - 1)$.

Expanding: $(k-1)(k^2 + 2k + 1) < k^3 + k^2 - k$.

Left side: $k^3 + 2k^2 + k - k^2 - 2k - 1 = k^3 + k^2 - k - 1$.

So we need: $k^3 + k^2 - k - 1 < k^3 + k^2 - k$, which is $-1 < 0$ $\checkmark$

Therefore, by mathematical induction, the inequality holds for all $n \ge 2$.
\end{solution}

\begin{takeaways}
\begin{itemize}
    \item Base case: Verify for smallest value ($n = 2$)
    \item Inductive step: Assume for $k$, prove for $k+1$
    \item Algebraic manipulation: Simplify the inequality to verify it holds
\end{itemize}
\end{takeaways}

