\begin{problem}[Weighted geometric sum]
Prove that for every integer $n\ge 1$,
\[
\sum_{k=1}^n k2^k = (n-1)2^{n+1}+2.
\]
\end{problem}

\begin{hint}
\begin{itemize}
  \item Verify the base case $n=1$ first.
  \item For induction, add the term $(m+1)2^{m+1}$ to the assumed sum for $m$.
  \item (Alternative) Differentiate the finite geometric series \(\sum_{k=0}^n x^k\) with respect to $x$ and substitute $x=2$. 
\end{itemize}
\end{hint}

\begin{solution}
\textbf{Induction.} For $n=1$ the left-hand side is $1\cdot2=2$ and the right-hand side is $(1-1)2^{2}+2=2$, so the base case holds.

Assume the identity holds for $n=m\ge1$. Then
\begin{align*}
\sum_{k=1}^{m+1} k2^k &= \left(\sum_{k=1}^m k2^k\right) + (m+1)2^{m+1} \\ 
&= (m-1)2^{m+1}+2 + (m+1)2^{m+1} \\ 
&= m2^{m+2}+2 = \bigl((m+1)-1\bigr)2^{(m+1)+1}+2,
\end{align*}
which is the desired formula for $n=m+1$. By induction the formula holds for all $n\ge1$.

\textbf{Proof with Calculus (Differentiation)} 

Consider the geometric series:
\[ P(x) = \sum_{k=0}^{n} x^k = \frac{x^{n+1}-1}{x-1} \]
Differentiating both sides with respect to $x$:
\[ \frac{d}{dx} \sum_{k=0}^{n} x^k = \sum_{k=1}^{n} k x^{k-1} \]
Using the quotient rule on the right-hand side:
\[ \sum_{k=1}^{n} k x^{k-1} = \frac{(n+1)x^n(x-1) - (x^{n+1}-1)}{(x-1)^2} \]
Multiply both sides by $x$ to obtain the desired summation form:
\[ \sum_{k=1}^{n} k x^k = \frac{(n+1)x^{n+1}(x-1) - x(x^{n+1}-1)}{(x-1)^2} \]
Substitute $x=2$:
\begin{align*}
    \sum_{k=1}^{n} k 2^k &= \frac{(n+1)2^{n+1}(2-1) - 2(2^{n+1}-1)}{(2-1)^2} \\
    &= (n+1)2^{n+1} - 2 \cdot 2^{n+1} + 2 \\
    &= 2^{n+1} (n+1-2) + 2 \\
    &= (n-1) 2^{n+1} + 2
\end{align*}
\qed
\end{solution}

\begin{takeaways}
\begin{itemize}
  \item Many weighted sums $\sum k a^k$ can be handled by induction or by differentiating a geometric series.
  \item Verifying base cases and clearly aligning the algebra in the inductive step keeps the argument clean for students.
\end{itemize}
\end{takeaways}
