% Part 2 Problem 06 (Medium): (2^m-1)^2 - 1 divisible by 2^{m+1}
% Source: samples/10.tex
% Technique: Direct Proof
% Topic: Divisibility/Exponents

\begin{problem}[Medium]
Prove that $(2^m - 1)^2 - 1$ is divisible by $2^{m+1}$ for all integers $m \geq 1$.
\end{problem}

\begin{hint}
Expand the perfect square $(2^m - 1)^2$ algebraically, then simplify. Try to factor out $2^{m+1}$ from the resulting expression.
\end{hint}

\begin{solutionsketch}
Let $E = (2^m - 1)^2 - 1$.

\textbf{Step 1:} Expand the square:
\begin{align*}
E &= (2^m)^2 - 2(2^m) + 1 - 1 \\
&= 2^{2m} - 2^{m+1} + 1 - 1 \\
&= 2^{2m} - 2^{m+1}
\end{align*}

\textbf{Step 2:} Factor out $2^{m+1}$:

Note that $2^{2m} = 2^{m+1} \cdot 2^{m-1}$ (using exponent laws).

Therefore:
\begin{align*}
E &= 2^{m+1} \cdot 2^{m-1} - 2^{m+1} \cdot 1 \\
&= 2^{m+1}(2^{m-1} - 1)
\end{align*}

\textbf{Step 3:} Conclude divisibility:

Since $m \geq 1$, we have $m - 1 \geq 0$, so $2^{m-1}$ is an integer. Thus $(2^{m-1} - 1)$ is an integer.

Therefore, $E = 2^{m+1} \cdot k$ where $k = 2^{m-1} - 1 \in \mathbb{Z}$.

By definition, $(2^m - 1)^2 - 1$ is divisible by $2^{m+1}$. $\qed$
\end{solutionsketch}
