% Part 2 Problem 14 (Hard): Inequality induction with sums of cubes
% Source: samples/27.tex
% Technique: Mathematical Induction (two inequalities)
% Topic: Induction/Inequalities

\begin{problem}[Hard]
Prove by induction that for all integers $n \geq 2$:
\[
1^3 + 2^3 + \cdots + (n-1)^3 < \frac{n^4}{4} < 1^3 + 2^3 + \cdots + n^3
\]
\end{problem}

\begin{hint}
This is a "sandwich" inequality with two parts:
\begin{itemize}
\item LHS inequality: $\sum_{k=1}^{n-1} k^3 < \frac{n^4}{4}$ (needs induction)
\item RHS inequality: $\frac{n^4}{4} < \sum_{k=1}^{n} k^3$ (can be proven directly)
\end{itemize}

Recall: $\sum_{k=1}^{n} k^3 = \left[\frac{n(n+1)}{2}\right]^2 = \frac{n^2(n+1)^2}{4}$

For the LHS induction step, you'll need to show $\frac{k^4}{4} + k^3 < \frac{(k+1)^4}{4}$, which simplifies to $0 < 6k^2 + 4k + 1$.
\end{hint}

\begin{solutionsketch}
\textbf{Part 1: RHS Inequality (Direct Proof)}

Show $\frac{n^4}{4} < \sum_{k=1}^{n} k^3$ for $n \geq 2$.

Using the sum formula:
\[
\sum_{k=1}^{n} k^3 = \frac{n^2(n+1)^2}{4} = \frac{n^4 + 2n^3 + n^2}{4}
\]

We need: $\frac{n^4}{4} < \frac{n^4 + 2n^3 + n^2}{4}$

This simplifies to: $0 < 2n^3 + n^2 = n^2(2n + 1)$

Since $n \geq 2 > 0$, this is clearly true. RHS proven. \checkmark

\vspace{0.5cm}

\textbf{Part 2: LHS Inequality (Induction)}

Prove $\sum_{k=1}^{n-1} k^3 < \frac{n^4}{4}$ for $n \geq 2$.

\vspace{0.3cm}

\textit{Base case ($n=2$):}
\[
\sum_{k=1}^{1} k^3 = 1^3 = 1 < \frac{2^4}{4} = 4 \quad \checkmark
\]

\vspace{0.3cm}

\textit{Inductive hypothesis:} Assume $\sum_{k=1}^{m-1} k^3 < \frac{m^4}{4}$ for some $m \geq 2$.

\vspace{0.3cm}

\textit{Inductive step:} Prove $\sum_{k=1}^{m} k^3 < \frac{(m+1)^4}{4}$.

\begin{align*}
\sum_{k=1}^{m} k^3 &= \sum_{k=1}^{m-1} k^3 + m^3 \\
&< \frac{m^4}{4} + m^3 \quad \text{(by IH)} \\
&= \frac{m^4 + 4m^3}{4}
\end{align*}

Need to show: $\frac{m^4 + 4m^3}{4} < \frac{(m+1)^4}{4}$

Equivalently: $m^4 + 4m^3 < (m+1)^4$

Expand RHS:
\[
(m+1)^4 = m^4 + 4m^3 + 6m^2 + 4m + 1
\]

So we need: $m^4 + 4m^3 < m^4 + 4m^3 + 6m^2 + 4m + 1$

Simplifies to: $0 < 6m^2 + 4m + 1$

This is true for all $m \geq 2$. \checkmark

\vspace{0.3cm}

By induction, LHS proven. Combining both parts, the full sandwich inequality holds. $\qed$
\end{solutionsketch}
